Sorting/QuicksortSpec.v
@@ -91,6 +91,46 @@ Proof.
           intros. apply uqs_In in H. eapply spec_lo; eauto.
 Qed.
 
+Inductive AllLess {A : Type} (R : A -> A -> Prop) (x : A) : list A -> Prop :=
+    | AllLess_nil : AllLess R x []
+    | AllLess_cons :
+        forall (h : A) (t : list A),
+          R x h -> AllLess R x t -> AllLess R x (h :: t).
+
+Inductive Sorted {A : Type} (R : A -> A -> Prop) : list A -> Prop :=
+    | Sorted_nil : Sorted R []
+    | Sorted_cons :
+        forall (h : A) (t : list A),
+          AllLess R h t -> Sorted R t -> Sorted R (h :: t).
+
+Theorem Sorted'_uqs :
+  forall
+    (A : LinDec) (small : Small A) (adhoc : AdHocSort small)
+    (choosePivot : Pivot A) (partition : Partition A) (l : list A),
+      Sorted A (uqs adhoc choosePivot partition l).
+Proof.
+  intros.
+  functional induction @uqs A small adhoc choosePivot partition l.
+    pose (e' := e). apply small_inl in e'; subst.
+      apply Sorted_adhoc in e. admit.
+    apply small_inr in e. apply pivot_spec in e0.
+      Check Sorted_app_all. ; auto.
+        apply Sorted_cons.
+          intros. apply in_app_or in H. destruct H.
+            erewrite spec_eq; eauto.
+            eapply spec_hi; eauto. eapply uqs_In; eauto.
+          apply Sorted_app; auto.
+            assert (forall x : A, In x eq -> x = pivot).
+              eapply spec_eq; eauto.
+              clear e1. induction eq; auto. destruct eq; auto. constructor.
+                rewrite (H a), (H c); cbn; auto.
+                apply IHeq. intro. inv 1; apply H; cbn; auto.
+            intros. apply uqs_In in H0.
+              erewrite (spec_eq pivot) at 1; eauto.
+                eapply spec_hi; eauto.
+          intros. apply uqs_In in H. eapply spec_lo; eauto.
+Qed.
+
 #[refine]
 Instance Sort_uqs
   (A : LinDec) (small : Small A) (adhoc : AdHocSort small)
