Thesis/Snippets/Chapter2/ImprovingPatchworkDefinitions.v
@@ -1,0 +1,29 @@
+Require Import List.
+Import ListNotations.
+
+Module M1.
+
+Inductive LessThanAll (n : nat) : list nat -> Prop :=
+    | LessThanAll_nil : LessThanAll n []
+    | LessThanAll_cons :
+        forall (h : nat) (t : list nat),
+          n <= h -> LessThanAll n t -> LessThanAll n (h :: t).
+
+Inductive Sorted : list nat -> Prop :=
+    | Sorted_nil : Sorted []
+    | Sorted_cons :
+        forall (h : nat) (t : list nat),
+          LessThanAll h t -> Sorted t -> Sorted (h :: t).
+
+End M1.
+
+Module M2.
+
+Inductive Sorted : list nat -> Prop :=
+    | Sorted_nil : Sorted []
+    | Sorted_singl : forall n : nat, Sorted [n]
+    | Sorted_cons :
+        forall (n m : nat) (l : list nat),
+          n <= m -> Sorted (m :: l) -> Sorted (n :: m :: l).
+
+End M2.
